Defs.v
@@ -12,6 +12,14 @@ Inductive multi {X} (R : relation X) : relation X :=
 
 Hint Constructors multi.
 
+Lemma multi_trans {X} (R : relation X) : forall x y z,
+  multi R x y -> multi R y z -> multi R x z.
+Proof.
+  induction 1.
+  * easy.
+  * intro. eapply multi_step; eauto.
+Qed.
+
 Definition normal_form {X} (R : relation X) (x : X) : Prop :=
   ~ exists y, R x y.
 
@@ -201,6 +209,7 @@ Fixpoint fill_context E M :=
   end
 where "E [ M ]" := (fill_context E M) : smallstep_scope.
 
+Delimit Scope smallstep_scope with smallstep.
 Open Scope smallstep_scope.
 
 Reserved Notation "M --> N" (at level 60).
